proved the desired bounds

CoRNMisc.v
@@ -30,17 +30,132 @@ Proof.
   - apply leEq_reflexive.
 Defined.
 
+
+
+Lemma cll : forall {a b}, a[<]b 
+  -> (clcr a b) a.
+intros ? ? Hlt. simpl.
+split.
+  - apply leEq_reflexive.
+  - apply less_leEq. trivial.
+Defined.
+
+Lemma clr : forall {a b}, a[<]b 
+  -> (clcr a b) b.
+intros ? ? Hlt. simpl.
+split.
+  - apply less_leEq. trivial.
+  - apply leEq_reflexive.
+Defined.
+
+Lemma clclLend : forall {a b} (cI : compact_ (clcr a b)),
+ Lend  cI = a.
+Proof.
+ simpl. reflexivity.
+Defined.
+
+Lemma clclRend : forall {a b} (cI : compact_ (clcr a b)),
+ Rend  cI = b.
+Proof.
+ simpl. reflexivity.
+Defined.
+
+Definition equivInterval (ia ib : interval) :=
+ forall x,  (ia x) IFF (ib x).
+
+Lemma derivContI' :
+forall {F F' : PartIR} {a b : IR}
+  {Hab : a [<] b}
+  (derivF : Derivative (clcr a b) Hab F F'),
+  Continuous_I (less_leEq _ _ _ Hab) F'.
+Proof.
+  intros.
+  apply Derivative_imp_Continuous' in derivF.
+  assert (compact_ (clcr a b)) as Ci
+     by (apply less_leEq; trivial).
+  apply Int_Continuous with (cI := Ci) (H:=less_leEq IR a b Hab) in derivF .
+  trivial.
+Defined.
+
+Lemma minmaxincluded: 
+forall a b (Hab : a [<] b),
+ included 
+     (Compact (Min_leEq_Max a b)) 
+     (Compact (less_leEq IR a b Hab)).
+Proof.
+ intros. unfold compact. simpl.
+ intros x Hc. destruct Hc as [Hcl Hcr].
+ apply less_leEq in Hab.
+ rewrite leEq_imp_Min_is_lft in Hcl;[| trivial].
+ rewrite leEq_imp_Max_is_rht in Hcr;[| trivial].
+ split; trivial.
+Qed.
+
+(** if we know that [a<b] many hypothesis in Barrow
+    can be removed *)
+Lemma Barrow2  : forall (F F' : PartIR) {a b : IR}
+  (Hab : a [<] b) (derivF : Derivative (clcr a b) Hab F F'),
+  let Hc := derivContI' derivF in
+  let Hb := Derivative_imp_inc _ _ _ _ derivF b (clr Hab) in
+  let Ha := Derivative_imp_inc _ _ _ _ derivF a (cll Hab) in 
+  integral a b (less_leEq _ _ _ Hab) F' Hc  [=]F b Hb[-]F a Ha.
+Proof.
+  intros.
+  assert (Continuous_I (Min_leEq_Max a b) F') as HF.
+  - eapply included_imp_contin; eauto.
+    apply minmaxincluded.
+  - rewrite <- Integral_integral with (HF := HF).
+    apply Barrow.
+    eapply Derivative_imp_Continuous';
+     eauto.
+Qed.
+
+Definition UBoundInCompInt {a b} (Hab : a [<]b)
+ (F : PartIR) (ub : IR) 
+   :=
+forall x : IR,
+  Compact (less_leEq IR a b Hab) x 
+  -> forall Hx : Dom F x, F x Hx[<=]ub.
+
+
+(** Combines Barrow's theorem ([Barrow2]) and 
+    [ub_integral]*)
 Lemma AntiderivativeUB : 
 forall (F F': PartFunct IR) (a b : IR) (Hab : a[<]b)
-     (derivF : Derivative_I Hab F F') (c : IR),
-     let HabC := (less_leEq IR a b Hab) in
-     let Hdb := (inDomDerRight derivF) in
-     let Hda := (inDomDerLeft derivF) in
-     fun_lub_IR F' (Compact HabC) c
+     (derivF : Derivative (clcr a b) Hab F F') (c : IR),
+     let Hdb := Derivative_imp_inc _ _ _ _ derivF b (clr Hab) in
+     let Hda := Derivative_imp_inc _ _ _ _ derivF a (cll Hab) in
+     UBoundInCompInt Hab F' c
      -> (F b Hdb[-] F a Hda)[<=]c[*](b[-]a).
 Proof.
-  intros ? ? ? ? ? ? ? ? ? ? Hlub.
+  intros ? ? ? ? ? ? ? ? ?  Hlub.
   subst Hda. subst Hdb.
-  unfold inDomDerRight.
-  unfold inDomDerLeft.
-  rewrite <- Barrow.
+  rewrite <- Barrow2.
+  apply ub_integral.
+ exact Hlub.
+Qed.
+
+Definition LBoundInCompInt {a b} (Hab : a [<]b)
+ (F : PartIR) (lb : IR) 
+   :=
+forall x : IR,
+  Compact (less_leEq IR a b Hab) x 
+  -> forall Hx : Dom F x, lb [<=] F x Hx.
+
+
+(** Combines Barrow's theorem ([Barrow2]) and 
+    [ub_integral]*)
+Lemma AntiderivativeLB : 
+forall (F F': PartFunct IR) (a b : IR) (Hab : a[<]b)
+     (derivF : Derivative (clcr a b) Hab F F') (c : IR),
+     let Hdb := Derivative_imp_inc _ _ _ _ derivF b (clr Hab) in
+     let Hda := Derivative_imp_inc _ _ _ _ derivF a (cll Hab) in
+     LBoundInCompInt Hab F' c
+     -> c[*](b[-]a) [<=] (F b Hdb[-] F a Hda).
+Proof.
+  intros ? ? ? ? ? ? ? ? ?  Hlub.
+  subst Hda. subst Hdb.
+  rewrite <- Barrow2.
+  apply lb_integral.
+ exact Hlub.
+Qed.
